EqType for values.

ifc/extended/Machine.v
@@ -973,10 +973,16 @@ Fixpoint fstepN t (n : nat) (s : State) : list State :=
 
 Import ssreflect ssrbool eqtype.
 
-Definition pc_eqP : Equality.axiom pc_eq.
+Lemma pc_eqP : Equality.axiom pc_eq.
 Proof. admit. Qed.
 
 Definition pc_eqMixin := EqMixin pc_eqP.
 Canonical pc_eqType := EqType _ pc_eqMixin.
+
+Lemma val_eqP : Equality.axiom val_eq.
+Proof. admit. Qed.
+
+Definition val_eqMixin := EqMixin val_eqP.
+Canonical val_eqType := EqType _ val_eqMixin.
 
 End MachineM.
